\documentclass{article}

\usepackage{amsmath,amsthm,amssymb}
\renewcommand{\qedsymbol}{$\blacksquare$}
\usepackage{soul}
\usepackage[T1]{fontenc}
\usepackage{titling}
\usepackage[left=3cm, right=3cm, top=2cm]{geometry}
\setlength{\droptitle}{0 em} 
\title{\textbf{NYU Computer Science Bridge HW6}\\
Summer 2023 Name: Jacky Choi}


\date{}
\begin{document}
\setul{}{2pt}
\maketitle

\noindent \textbf{Question 5}\\\\
\textbf{Use the definition of $\theta$ in order to show the following: }\\\\
\textbf{a.}
$5n^3 + 2n^2 + 3n = \theta (n^3)$\\\\
\begin{proof}

Assume $n > 0$, then $5n^3 + 2n^2 + 3n \leq 5n^3 + 2n^3 + 3n^3$\\
$5n^3 + 2n^2 + 3n \leq 10n^3$\\
$5n^3 < 5n^3 + 2n^2 + 3n$\\
$5n^3 + 2n^2 + 3n = \theta(n^3)$
\end{proof}
\noindent \textbf{b.}
$\sqrt{7n^2 + 2n - 8} = \theta (n)$\\\\
\begin{proof}

    Assume $n > 4$, then $\sqrt{7n^2 + 2n - 8} < \sqrt{7n^2 + 2n^2}$\\
    $\sqrt{7n^2 + 2n^2} < \sqrt{3n^2} = 3n$\\
    and $\sqrt{7n^2 + 2n^2 - 8} > \sqrt{7n^2} = 7x$\\
    then $\sqrt{7n^2 + 2n^2 - 8} = \theta(n)$
    \end{proof}
\end{document}